src/Misc.v
@@ -4,3 +4,8 @@ From Coq Require Import Morphisms Arith.
 Proof.
   unfold Proper, respectful; intros; apply Nat.add_le_mono; assumption.
 Qed.
+
+#[global] Instance Proper_sub_le : Proper (le ==> eq ==> le) Nat.sub.
+Proof.
+  unfold Proper, respectful; intros; subst; apply Nat.sub_le_mono_r; assumption.
+Qed.
